\textbf{\Large The Derivability Conditions}
\ \\
\ \\
\begin{theorem}{Proposition}
Course-of-Values Induction
\end{theorem}\\
\begin{theorem}{Proposition}
The Least Principle
\end{theorem}\\
\begin{theorem}{Lemma}
\[
\Phi_\pa \derives (\varphi_{div}(x, y) \land 0 < y) \limply x \leq y.
\]
\end{theorem}
\begin{theorem}{Lemma}
\[
\Phi_\pa \derives (\varphi_{prime}(x) \land \varphi_{div}(x, y \mul z) \land 0 < y \mul z) \limply (\varphi_{div}(x, y) \lor \varphi_{div}(x, z)).
\]
\end{theorem}
\begin{theorem}{Lemma}
\[
\Phi_\pa \derives exp(2, x + 1) \geq 2.
\]
\end{theorem}
\begin{theorem}{Lemma}
\[
\Phi_\pa \derives sub(exp(2, x + 1), 2) + 2 \equal exp(2, x + 1).
\]
\end{theorem}
\begin{theorem}{Lemma}
\[
\Phi_\pa \derives ((\varphi_{prime}(y) \land \varphi_{div}(y, exp(2, x + 1))) \limply y \equal 2).
\]
\end{theorem}
\begin{theorem}{Lemma A}
\[
\Phi_\pa \derives leng(seq(x)) \equal 1.
\]
\end{theorem}
\begin{theorem}{Lemma B}
\[
\Phi_\pa \derives leng(concat(x, y)) \equal leng(x) + leng(y).
\]
\end{theorem}
\begin{theorem}{Lemma C}
\[
\Phi_\pa \derives (\forall k < leng(x))index(concat(x, y), k) \equal index(x, k)
\]
and
\[
\Phi_\pa \derives (\forall k < leng(y))index(concat(x, y), leng(x) + k) \equal index(y, k).
\]
\end{theorem}
\begin{theorem}{Lemma D}
\[
\Phi_\pa \derives P_\ant(x, sqnt(union(ant(x), y), suc(x))).
\]
\end{theorem}
\begin{theorem}{Lemma E}
\[
\Phi_\pa \derives P_{mp}(sqnt(x, imp(y, z)), sqnt(x, y), sqnt(x, z)).
\]
\end{theorem}
\begin{theorem}{Lemma F}
\[
\Phi_\pa \derives suc(sqnt(x, y)) \equal y.
\]
\end{theorem}
\begin{theorem}{Lemma G}
\[
\Phi_\pa \derives ant(sqnt(x, y)) \equal x.
\]
\end{theorem}
\begin{theorem}{Lemma H}
\[
\Phi_\pa \derives (\varphi_{dvn}(x) \land \varphi_{dvn}(y)) \limply \varphi_{dvn}(concat(x, y)).
\]
\end{theorem}
\begin{theorem}{Lemma I}
\[
\Phi_\pa \derives (\forall z < union(x, y))(\varphi_\in(z, union(x, y)) \limply (\varphi_\in(z, x) \lor \varphi_\in(z, y))).
\]
\end{theorem}
\begin{theorem}{Lemma}
\[
\Phi_\pa \derives (\varphi_H(u, x) \land \varphi_H(imp(u, v), y)) \limply \varphi_H(v, t_3)
\]
where
\[
\begin{array}{lll}
t_0 & = & concat(x, y), \cr
t_1 & = & concat(t_0, seq(sqnt(union(ant(last(x)), ant(last(y))), u))), \cr
t_2 & = & concat(t_1, seq(sqnt(union(ant(last(x)), ant(last(y))), imp(u, v)))), \cr
t_3 & = & concat(t_2, seq(sqnt(union(ant(last(x)), ant(last(y))), v))).
\end{array}
\]
\end{theorem}
\begin{proof} (INCOMPLETE)\\
We get:
\begin{enumerate}[(1)]
%
\item $\Phi_\pa \derives leng(t_3) \equal leng(x) + leng(y) + 3$ from Lemmas A and B;
%
\item By Lemma C, we have
\[
\Phi_\pa \derives index(t_3, leng(x) - 1) \equal last(x)
\]
and
\[
\Phi_\pa \derives index(t_3, leng(x) + leng(y)) \equal seq(sqnt(union(ant(last(x)), ant(last(y))), u)).
\]
Also,
\[
\Phi_\pa \setsum \setenum{\varphi_H(u, x)} \derives suc(last(x)) \equal u.
\]
Therefore, by Lemma D we conclude
\[
\Phi_\pa \setsum \setenum{\varphi_H(u, x), \varphi_H(imp(u, v), y)} \derives P_\ant(index(t_3, leng(x) - 1), index(t_3, leng(x) + leng(y))).
\]
%
\item By Lemma C, we have
\[
\Phi_\pa \derives index(t_3, leng(x) + leng(y) - 1) \equal last(y)
\]
and
\[
\Phi_\pa \derives index(t_3, leng(x) + leng(y) + 1) \equal seq(sqnt(union(ant(last(x)), ant(last(y))), imp(u, v))).
\]
Also,
\[
\Phi_\pa \setsum \setenum{\varphi_H(imp(u, v), y)} \derives suc(last(y)) \equal imp(u, v).
\]
Therefore, by Lemma D we conclude
\[
\Phi_\pa \setsum \setenum{\varphi_H(u, x), \varphi_H(imp(u, v), y)} \derives P_\ant(index(t_3, leng(x) + leng(y) - 1), index(t_3, leng(x) + leng(y) + 1)).
\]
%
\item By Lemma C, we have
\[
\Phi_\pa \derives index(t_3, leng(x) + leng(y)) \equal seq(sqnt(union(ant(last(x)), ant(last(y))), u)),
\]
\[
\Phi_\pa \derives index(t_3, leng(x) + leng(y) + 1) \equal seq(sqnt(union(ant(last(x)), ant(last(y))), imp(u, v)))
\]
and
\[
\Phi_\pa \derives seq(sqnt(union(ant(last(x)), ant(last(y))), v)).
\]
Using Lemma E, we therefore conclude
\[
\Phi_\pa \setsum \setenum{\varphi_H(u, x), \varphi_H(imp(u, v), y)} \derives P_{mp}(index(t_3, leng(x) + leng(y) + 1), index(t_3, leng(x) + leng(y)), index(t_3, leng(x) + leng(y) + 2)).
\]
%
\item Using (1) and Lemmas C and F, we obtain
\[
\Phi_\pa \setsum \setenum{\varphi_H(u, x), \varphi_H(imp(u, v), y)} \derives suc(last(t_3)) \equal v.
\]
%
\item Using (1), (2), (3), (4) and Lemmas C, H, I, we obtain
\[
\Phi_\pa \setsum \setenum{\varphi_H(u, x), \varphi_H(imp(u, v), y)} \derives \varphi_{dvn\Phi}(t_3).
\]
%
\end{enumerate}
Thus,
\[
\Phi_\pa \setsum \setenum{\varphi_H(u, x), \varphi_H(imp(u, v), y)} \derives \varphi_H(v, t_3)
\]
and
\[
\Phi_\pa \derives (\varphi_H(u, x) \land \varphi_H(imp(u, v), y)) \limply \varphi_H(v, t_3). \qedhere
\]
\end{proof}
(HERE)\\
\ \\
\textbf{Lemma.} $\Phi_\pa \vdash (P_{Dvn} (v_0) \land P_{Dvn} (v_1)) \rightarrow P_{Dvn} (v_0 \ast v_1)$.\\
\ \\
\textit{Proof.} It suffices to show
\[
\Phi_\pa \cup \{ P_{Dvn} (v_0), P_{Dvn} (v_1) \} \vdash P_{Dvn} (v_0 \ast v_1).
\]
By II.2.21 (p.247) we have
\[
\begin{array}{l}
\Phi_\pa \cup \{ P_{Dvn} (v_0), P_{Dvn} (v_1) \} \vdash P_{Seq} (v_0 \ast v_1),\cr
\Phi_\pa \cup \{ P_{Dvn} (v_0), P_{Dvn} (v_1) \} \vdash Length(v_0 \ast v_1) \equiv Length(v_0 + v_1).
\end{array}
\]
Hence
\[
\Phi_\pa \cup \{ P_{Dvn} (v_0), P_{Dvn} (v_1) \} \vdash P_{Seq} (v_0 \ast v_1) \land 0 < Length(v_0 \ast v_1).
\]
Again by II.2.21,
\[
\begin{array}{l}
\Phi_\pa \vdash (\forall i < Length(v_0))(v_0 \ast v_1)[i] \equiv v_0[i],\cr
\Phi_\pa \vdash (\forall i < Length(v_1))(v_0 \ast v_1)[i + Length(v_0] \equiv v_1[i].
\end{array}
\]
\ \\
\textbf{Lemma.} $\Phi_\pa \vdash (P_{Dvn} (v_0) \land (\exists k < Length(v_0)) P_\ant (v_1, v_0[k])) \rightarrow P_{Dvn} (v_0 \ast \langle v_1 \rangle)$.\\
\ \\
\textit{Proof.}\\
\ \\
\textbf{Lemma.} $(P_{Dvn} (v_0) \land (\exists i < Length(v_0))(\exists j < Length(v_0))P_{Mp} (v_1, v_0[i], v_0[j]))$ $\rightarrow P_{Dvn} (v_0 \ast \langle v_1 \rangle)$.\\
%Space consideration
\ \\
\textit{Proof.}\\
\ \\
\textbf{Lemma.} 
\[
\begin{array}{l}
\Phi_\pa \vdash (\varphi_H (v_0, u_0) \land \varphi_H (4\pi (4v_0 + 1, v_1) + 2, u_1)) \rightarrow\cr
\phantom{\Phi_\pa \vdash (} \varphi_H (v_1, u_0 \ast u_1 \ast \langle \pi (\pi_1 (Last(u_0)) \cup \pi_1 (Last(u_1)), v_0) \rangle\cr
\phantom{\Phi_\pa \vdash (\varphi_H (v_1, u_0 \ast u_1} \ast \langle \pi (\pi_1 (Last(u_0)) \cup \pi_1 (Last(u_1)), 4\pi (4v_0 + 1, v_1) + 2) \rangle\cr
\phantom{\Phi_\pa \vdash (\varphi_H (v_1, u_0 \ast u_1} \ast \langle \pi (\pi_1 (Last(u_0)) \cup \pi_1 (Last(u_1)), v_1) \rangle
).
\end{array}
\]
\ \\
\textit{Proof.}\\
\ \\
\textbf{Corollary.} (The Derivability Condition (L2)) \emph{Let $\Phi \supset \Phi_\pa$ be decidable. Then for all $S_\ar$-formulas $\varphi$ and $\psi$,
\[
\Phi_\pa \vdash (\Der{\Phi} (\mbf{n}^\varphi ) \land \Der{\Phi} (\mbf{n}^{(\varphi \rightarrow \psi )})) \rightarrow \Der{\Phi} (\mbf{n}^\psi ).
\]}